---
layout: post
title: 3-2-7
date: '2023-01-20 01:17:09 +0800'
categories: [Introduction to algorithm 3th]
tags: [Algorithms]
usemathjax: true
---
# Problem
> Prove by induction that the $i$th Fibonacci number satisfies the equality
> \begin{equation}
>   F_i= \frac{\phi^i-\hat{\phi}^i}{\sqrt{5}},
> \end{equation}
> where $\phi$ is the golden ratio and $\hat{\phi}$​ is its conjugate.(two roots of the equation）
> \begin{equation}
>   x^2 = x + 1
> \end{equation}


# Proof
-   Base case: 

    For $i=0,$
    \begin{equation}
    \begin{aligned}
    \frac{\phi^0-\hat{\phi}^0}{\sqrt{5}} &= \frac{1-1}{\sqrt{5}} \newline 
      &= 0 \newline 
      &= F_0.
    \end{aligned}
    \end{equation}

    For $i=1,$
    \begin{aligned}
    \frac{\phi^1-\hat{\phi}^1}{\sqrt{5}} &= \frac{(1+\sqrt{5})-(1-\sqrt{5})}{2\sqrt{5}} \newline 
      &= 1 \newline 
      &= F_1.
    \end{aligned}

-   Induction step: 
    Suppose $i=k,$

    -    $  
         F_k = \frac{\phi^k-\hat{\phi}^k}{\sqrt{5}},
         \tag{1}
         $

    -    $
         F_{k-1} = \frac{\phi^{k-1}-\hat{\phi}^{k-1}}{\sqrt{5}}and
         \tag{3}
         $

    -    $
         F_{k+1} = \frac{\phi^{k+1}-\hat{\phi}^{k+1}}{\sqrt{5}}
         \tag{2}
         $

    \begin{aligned}
    F_{k-1} + F_{k} &= \frac{\phi^{k-1}-\hat{\phi}^{k-1}}{\sqrt{5}} + \frac{\phi^{k}-\hat{\phi}^{k}}{\sqrt{5}} \newline 
      &= \frac{\phi^{k-1}(1+\phi) - \hat{\phi}^{k-1}(1+\hat{\phi})}{\sqrt{5}}
    \end{aligned}

    Because $\phi$ and $\hat{\phi}$ are two roots of $ x^2 = x + 1$, above equation can be written as

    \begin{aligned}
    \frac{\phi^{k-1} \cdot \phi^2 - \hat{\phi}^{k-1} \cdot \hat{\phi}^2}{\sqrt{5}} &= \frac{\phi^{k+1} - \hat{\phi}^{k+1}}{\sqrt{5}} \newline 
     &= F_{k+1}. 
    \end{aligned}
  <p align="right">$\blacksquare$</p>
  
# References
1. [Proof-by-induction](https://walkccc.me/CLRS/Chap03/3.2/#32-7)